code/hash/Hacl.Hash.MD.fsti
@@ -4,13 +4,13 @@ open Hacl.Hash.Definitions
 open Spec.Hash.Definitions
 
 noextract inline_for_extraction
-val mk_update_multi: a:hash_alg -> update:update_st a -> update_multi_st a
+val mk_update_multi: a:hash_alg{is_md a} -> update:update_st a -> update_multi_st a
 
 noextract inline_for_extraction
-val mk_update_last: a:hash_alg -> update_multi_st a -> pad_st a -> update_last_st a
+val mk_update_last: a:hash_alg{is_md a} -> update_multi_st a -> pad_st a -> update_last_st a
 
 noextract inline_for_extraction
-val mk_hash: a:hash_alg ->
+val mk_hash: a:hash_alg{is_md a} ->
   alloca:alloca_st a ->
   update_multi:update_multi_st a ->
   update_last:update_last_st a ->
